Proving ProgramLogic.v

platform/cito/ProgramLogic.v
@@ -7,14 +7,123 @@ Module Make (Import E : ADT).
   Require Import Semantics.
   Module Import SemanticsMake := Make E.
 
-  Definition Assert := State -> Prop.
+  Section TopSection.
 
-  Require Import Syntax Notations3.
+    Require Import Syntax Notations3.
 
-  Fixpoint wp stmt (a : Assert) : Assert :=
-    match stmt with
-      | x <- e => Subst a x e
-      | a ;; b => wp a (wp b a)
-      | If e {t} else {f} => (b /\ wp t a) \/ (~ b /\ wp f a)
-      | [I] While (e) {{ body }} => I
-      | DCall f ( args ) => 
+    (* shallow embedding *)
+    Definition assert := State -> Prop.
+    Definition interp (p : assert) (s : State) : Prop := p s.
+    Definition abs (f : State -> Prop) : assert := f.
+
+    Inductive StmtEx := 
+    | SkipEx : StmtEx
+    | SeqEx : StmtEx -> StmtEx -> StmtEx
+    | IfEx : Expr -> StmtEx -> StmtEx -> StmtEx
+    | WhileEx : assert -> Expr -> StmtEx -> StmtEx
+    | AssignEx : string -> Expr -> StmtEx.
+
+    Definition and_lift (a b : assert) : assert := abs (fun s => interp a s /\ interp b s).
+    Definition or_lift (a b : assert) : assert := abs (fun s => interp a s \/ interp b s).
+    Definition imply_close (a b : assert) : Prop := forall s, interp a s -> interp b s.
+
+    Infix "/\" := and_lift : assert_scope.
+    Infix "\/" := or_lift : assert_scope.
+    Infix "-->" := imply_close (at level 90) : assert_scope.
+
+    Require Import SemanticsExpr.
+
+    Close Scope equiv_scope.
+
+    Definition is_true e : assert := abs (fun s => eval (fst s) e <> $0).
+    Definition is_false e : assert := abs (fun s => eval (fst s) e = $0).
+
+    Open Scope assert_scope.
+
+    Fixpoint sp (stmt : StmtEx) (p : assert) : assert :=
+      match stmt with
+        | SkipEx => p
+        | SeqEx a b => sp b (sp a p)
+        | IfEx e t f => sp t (p /\ is_true e) \/ sp f (p /\ is_false e)
+        | WhileEx inv e _ => inv /\ is_false e
+        | AssignEx x e => 
+          abs (fun s => 
+                 exists w, 
+                   let s' := (upd (fst s) x w, snd s) in
+                   interp p s' /\
+                   sel (fst s) x = eval (fst s') e)%type
+      end.
+
+    Fixpoint vc stmt (p : assert) : list Prop :=
+      match stmt with
+        | SkipEx => nil
+        | SeqEx a b => vc a p ++ vc b (sp a p)
+        | IfEx e t f => vc t (p /\ is_true e) ++ vc f (p /\ is_false e)
+        | WhileEx inv e body => 
+          (p --> inv) :: (sp body (inv /\ is_true e) --> inv) :: vc body (inv /\ is_true e)
+        | AssignEx x e => nil
+      end.
+    
+    Fixpoint to_stmt s :=
+      match s with
+        | SkipEx => Syntax.Skip
+        | SeqEx a b => Syntax.Seq (to_stmt a) (to_stmt b)
+        | IfEx e t f => Syntax.If e (to_stmt t) (to_stmt f)
+        | WhileEx _ e b => Syntax.While e (to_stmt b)
+        | AssignEx x e => Syntax.Assign x e
+      end.
+
+    Coercion to_stmt : StmtEx >-> Stmt.
+
+    Definition and_all := fold_right and True.
+
+    Theorem sound' : forall env (s : Stmt) v v', RunsTo env s v v' -> forall s' : StmtEx, s = s' -> forall p, and_all (vc s' p) -> interp p v -> interp (sp s' p) v'.
+      induction 1; simpl; intros; destruct s'; try discriminate; simpl in *; try (injection H1; intros; subst).
+
+      (* skip *)
+      eauto.
+
+      (* seq *)
+      Lemma and_all_app : forall ls1 ls2, and_all (ls1 ++ ls2) -> and_all ls1 /\ and_all ls2.
+        admit.
+      Qed.
+      Require Import GeneralTactics.
+      eapply and_all_app in H2; openhyp.
+      eauto.
+
+      (* if *)
+      eapply and_all_app in H2; openhyp.
+      Lemma is_true_intro : forall e v, wneb (eval (fst v) e) $0 = true -> interp (is_true e) v.
+        admit.
+      Qed.
+      Hint Resolve is_true_intro.
+      Lemma is_false_intro : forall e v, wneb (eval (fst v) e) $0 = false -> interp (is_false e) v.
+        admit.
+      Qed.
+      Hint Resolve is_false_intro.
+      left.
+      eapply IHRunsTo; eauto.
+      split; eauto.
+
+      eapply and_all_app in H2; openhyp.
+      right.
+      eapply IHRunsTo; eauto.
+      split; eauto.
+
+      (* while *)
+      subst loop.
+      injection H2; intros; subst.
+      openhyp.
+      (*here*)
+      eapply IHRunsTo2.
+      inversion H.
+      subst loop0 loop1.
+      subst.
+
+    Qed.
+
+    Theorem sound : forall env (s : StmtEx) v v', RunsTo env s v v' -> forall p, and_all (vc s p) -> interp p v -> interp (sp s p) v'.
+
+  End TopSection.
+
+End Make.
